\documentclass{article}

\usepackage[margin=1in]{geometry}

\usepackage{amsmath}
\usepackage{amssymb}
\usepackage{arydshln}
\usepackage{calc}
\usepackage{enumitem}
\usepackage{lmodern}
\usepackage{mathtools}
\usepackage{pgfplots}
\usepackage{qtree}
\usepackage{slashed}
\usepackage{upgreek}
\usepackage{xfrac}
\usepackage[normalem]{ulem}
\usepackage[utf8]{inputenc}
\usepackage[T1]{fontenc}
\usepackage[hidelinks]{hyperref}

\begin{document}


\section{Determinante $A_{(n \times n)}$}

\bigbreak
$A_{1x1} = [a] \ \ \ \ \ \ det(A) = a$
\bigbreak
$A_{2 \times 2} = 
\begin{bmatrix}
    a_{11} & a_{12} \\
    a_{21} & a_{22} \\
\end{bmatrix} \ \ \ \ 
det(A) = a_{11} \cdot a_{22} - a_{12} \cdot a_{21}$

\bigbreak

$A_{3 \times 3} = 
\begin{bmatrix}
    a_{11} & a_{12} & a_{13} \\
    a_{21} & a_{22} & a_{23} \\  
    a_{31} & a_{32} & a_{33} \\  

\end{bmatrix}
$ \bigbreak
Cofator $a_{ij} = (-1)^{i + j} \ \cdot \ detÃ_{ij} $

$ã_{21} = (-1)^{2+1} \cdot det
 \begin{bmatrix}
    a_{12} & a_{13} \\
    a_{32} & a_{33} \\
 \end{bmatrix}$
\bigbreak
$det (A) = $ a soma dos produtos dos elementos de uma linha da matriz pelos 
seus cofatores = $a_{21} \cdot ã_{21} + a_{22} \cdot ã_{22} + a_{23} \cdot ã_{23} +$


$B =
\begin{bmatrix}
    1 & 2 & 3 \\
    -1 & 3 & 2 \\
    2 & 1 & -2 \\
\end{bmatrix}
$ \bigbreak
$ã_{11} = (-1)^{1+1} \cdot det
\begin{bmatrix}
    3 & 2 \\
    1 & -2 \\
\end{bmatrix}$
$=-8$ \bigbreak
$ã_{12} = (-1)^{1+2} \cdot det
\begin{bmatrix}
    -1 & 2 \\
    2 & -2 \\
\end{bmatrix}$
$=-[-2] = 2$ \bigbreak

$ã_{13} = (-1)^{1+3} \cdot det
\begin{bmatrix}
    -1 & 3 \\
    2 & 1 \\
\end{bmatrix}$
$=-7$
\bigbreak

$det(B) = 1 \cdot (-8) + 2 \cdot (2) + 3\cdot (-7)$

$= -7$

\bigbreak

$C = \begin{bmatrix}
    1 & 2 & 3 & 4 \\
    0 & 0 & 0 & -3 \\
    -1 & 3 & 2 & 5 \\
    2 & 1 & -2 & 0 \\
\end{bmatrix}$
\bigbreak
$det C =$ \bigbreak
$ã_{24} = (-1)^{2+4} \cdot det \begin{bmatrix}
    1 & 2 & 3 \\
    -1 & 3 & -2 \\
    2 & 1 & -2 \\
\end{bmatrix} = -25$

\bigbreak

$A = \begin{bmatrix}
    a_{11} & 0 & 0 & 0 \\
    a_{21} & a_{22} & 0 & 0 \\
    a_{31} & a_{32} & a_{34} & 0 \\
    a_{41} & a_{42} & a_{43} & a_{44} \\
\end{bmatrix}$
\bigbreak
$det(A) = a_{11} \cdot ã_{11} = a_{11} \cdot (-1)^{1+1} \cdot det \begin{bmatrix}
    a_{22} & 0 & 0 \\
    a_{32} & a_{33} & 0 \\
    a_{42} & a_{43} & a_{44} \\
\end{bmatrix}$
\bigbreak
$a_{11} \cdot [a_{11} ã_{22}] = a_{11} a_{22} \cdot (-1)^{2+2} det \begin{bmatrix}
    a_{33} & 0 \\
    a_{430} & a_{44} \\
\end{bmatrix} = a_{11}\cdot a_{22}\cdot a_{33}\cdot a_{44}$

\bigbreak

$A = \begin{bmatrix}
    1 & 2 \\
    -1 & 0 \\
\end{bmatrix}
$ \bigbreak $det A = 2$

$B = \begin{bmatrix}
    0 & 1 \\
    2 & 1 \\
\end{bmatrix}
$
\bigbreak $det B = -2$

$A + B = \begin{bmatrix}
    1 & 3 \\
    1 & 1 \\
\end{bmatrix}$
\bigbreak $det (A + B) = 2$
\bigbreak $det (A + B) \neq det(A) + det(B)$

\bigbreak

$det \begin{bmatrix}
    A_1 \\
    A_2 \\
    \vdots \\
    \alpha x + \beta y \\
    \vdots \\
    A_n
\end{bmatrix} = det \begin{bmatrix}
    A_1 \\
    \vdots \\
    \alpha x \\
    \vdots \\
    A_n
\end{bmatrix} + det \begin{bmatrix}
    A_1 \\
    \vdots \\
    \beta y \\
    \vdots \\
    A_n
\end{bmatrix} = \alpha \cdot det \begin{bmatrix}
    A_1 \\
    \vdots \\
    x\\
    \vdots \\
    A_n
\end{bmatrix} = \beta \cdot det \begin{bmatrix}
    A_1 \\
    \vdots \\
    y\\
    \vdots \\
    A_n
\end{bmatrix}$

\bigbreak

$det = \begin{bmatrix}
    \cos t & \sin t \\
    2\cos t -3 \sin t & \sin t + 3 \cos t\\
\end{bmatrix}$

\bigbreak
 
$ = det \begin{bmatrix}
    \cos t && \sin t \\
    2\cos t && 2\sin t \\
\end{bmatrix}
+ det \begin{bmatrix}
    \cos t && \sin t \\
    -3\sin t && 3\cos t \\
\end{bmatrix} = 
$\bigbreak

$2 \cdot det \begin{bmatrix}
    \cos t && \sin t \\
    \cos t && \sin t \\
\end{bmatrix}
+ 3\cdot det\begin{bmatrix}
    \cos t && \sin t \\
    -\sin t && \cos t \\
\end{bmatrix} 
= 2\cdot 0 + 3 \cdot 1 = 3
$


$A = \begin{bmatrix}
    1 & 2 \\
    -1 & 0 \\
\end{bmatrix}
$ \bigbreak $det A = 2$
\bigbreak

$B = \begin{bmatrix}
    0 & 1 \\
    2 & 1 \\
\end{bmatrix}
$
\bigbreak $det B = -2$

$A \cdot B = \begin{bmatrix}
    4 & 3 \\
    0 & -1 \\
\end{bmatrix}
$

\bigbreak

$det ( A \cdot B ) = -4 = det(A) \cdot det(B)$

\bigbreak

$A^t  = \begin{bmatrix}
    1 & -1 \\
    2 & 0 \\
\end{bmatrix}
$
\bigbreak
$det (A^t) = 2$
\bigbreak
$detA = det(A^t)$





\end{document}